STerm.v
@@ -1,0 +1,1096 @@
+Require Import List.
+Require Import Arith.
+Require Import Freevar.
+Require Import Misc.
+Require Import Psatz.
+
+Definition renaming := list nat.
+Fixpoint renv (L : renaming) (n : nat) : nat :=
+  match L with
+  | nil => n
+  | k :: L => if le_lt_dec k n then S (k + renv L (n - k)) else n
+  end.
+Lemma renv_car : forall L, { C | (forall n, renv L n < renv L (S n)) /\ (forall n, renv L (n + C) = n + renv L C) }.
+Proof.
+  induction L as [|k L].
+  - exists 0. split.
+    + intros n. simpl. constructor.
+    + intros n. simpl. reflexivity.
+  - destruct IHL as (C & HC1 & HC2).
+    exists (k + C). split.
+    + intros n. unfold renv; fold renv.
+      repeat destruct le_lt_dec.
+      * apply lt_n_S. apply plus_lt_compat_l.
+        replace (S n - k) with (S (n - k)); [apply HC1|].
+        apply minus_Sn_m. assumption.
+      * lia.
+      * lia.
+      * lia.
+    + intros. simpl.
+      repeat (destruct le_lt_dec; try lia).
+      replace (n + (k + C) - k) with (n + C) by lia.
+      replace (k + C - k) with C by lia.
+      rewrite HC2. lia.
+Defined.
+
+Lemma renv_add : forall k, { L | forall n, renv L n = k + n }.
+Proof.
+  induction k as [|k].
+  - exists nil. simpl. reflexivity.
+  - destruct IHk as (L & HL). exists (0 :: L). intros. simpl.
+    f_equal. rewrite HL. lia.
+Defined.
+
+Definition plus_ren k := proj1_sig (renv_add k).
+Definition plus_ren_correct k : forall n, renv (plus_ren k) n = k + n := proj2_sig (renv_add k).
+
+Lemma f_strict_mono_le : forall f, (forall n, f n < f (S n)) -> (forall n, n <= f n).
+Proof.
+  intros. induction n as [|n].
+  - lia.
+  - specialize (H n). lia.
+Qed.
+
+Lemma f_strict_mono_f0 : forall f, (forall n, f n < f (S n)) -> (forall n, f 0 <= f n).
+Proof.
+  intros. induction n as [|n].
+  - lia.
+  - specialize (H n). lia.
+Qed.
+
+Lemma f_strict_mono : forall f, (forall n, f n < f (S n)) -> (forall n m, n < m -> f n < f m).
+Proof.
+  intros f H n m Hlt. induction Hlt.
+  - apply H.
+  - specialize (H m). lia.
+Qed.
+
+Lemma renv_repeat0 : forall k L n, renv (repeat 0 k ++ L) n = k + renv L n.
+Proof.
+  induction k as [|k].
+  - intros. simpl. reflexivity.
+  - intros. simpl. rewrite IHk. f_equal. f_equal. f_equal. lia.
+Qed.
+
+Definition lift (L : renaming) : renaming :=
+  match L with
+  | nil => nil
+  | k :: L => S k :: L
+  end.
+
+Lemma lift_renv :
+  forall n L, renv (lift L) n = match n with 0 => 0 | S n => S (renv L n) end.
+Proof.
+  intros [|n] [|k L]; try reflexivity.
+  unfold lift. unfold renv; fold renv.
+  repeat destruct le_lt_dec; try lia.
+  reflexivity.
+Qed.
+
+Lemma renv_uncar :
+  forall f, { C | (forall n, f n < f (S n)) /\ (forall n, f (n + C) = n + f C) } -> { L | forall n, renv L n = f n }.
+Proof.
+  intros f (C & HC1 & HC2). revert f HC1 HC2; induction C as [|C]; intros f HC1 HC2.
+  - exists (proj1_sig (renv_add (f 0))). intros n.
+    destruct renv_add as (L & HL). simpl. rewrite HL.
+    specialize (HC2 n). rewrite <- plus_n_O in HC2. lia.
+  - specialize (IHC (fun n => f (S n) - S (f 0))). simpl in IHC.
+    destruct IHC as (L & HL).
+    + intros. assert (H := HC1 (S n)). assert (H2 := f_strict_mono_f0 f HC1 n). specialize (HC1 n). lia.
+    + intros. rewrite plus_n_Sm, HC2. assert (H := f_strict_mono_f0 f HC1 C). specialize (HC1 C). lia.
+    + exists (repeat 0 (f 0) ++ lift L). intros [|n]; rewrite renv_repeat0, lift_renv; simpl.
+      * lia.
+      * rewrite HL. assert (H := HC1 n). assert (H2 := f_strict_mono_f0 f HC1 n). lia.
+Defined.
+
+Lemma renv_comp_def :
+  forall L1 L2, { L3 | forall n, renv L3 n = renv L1 (renv L2 n) }.
+Proof.
+  intros L1 L2. apply renv_uncar.
+  destruct (renv_car L1) as (C1 & HC1a & HC1b).
+  destruct (renv_car L2) as (C2 & HC2a & HC2b).
+  exists (C1 + C2). split.
+  - intros n. apply f_strict_mono; [assumption|]. apply HC2a.
+  - intros n. rewrite Nat.add_assoc, !HC2b.
+    rewrite Nat.add_comm with (n := C1), HC1b.
+    rewrite Nat.add_comm, Nat.add_assoc, HC1b. lia.
+Defined.
+
+Definition renv_comp L1 L2 := proj1_sig (renv_comp_def L1 L2).
+Definition renv_comp_correct L1 L2 : forall n, renv (renv_comp L1 L2) n = renv L1 (renv L2 n) := proj2_sig (renv_comp_def L1 L2).
+
+
+
+
+
+
+
+Inductive term :=
+| var : nat -> term
+| abs : term -> term
+| app : term -> term -> term.
+
+Fixpoint ren (r : renaming) t :=
+  match t with
+  | var n => var (renv r n)
+  | abs t => abs (ren (lift r) t)
+  | app t1 t2 => app (ren r t1) (ren r t2)
+  end.
+
+Fixpoint subst t k u :=
+  match t with
+  | var n => if Nat.eq_dec k n then u else var n
+  | abs t => abs (subst t (S k) (ren (plus_ren 1) u))
+  | app t1 t2 => app (subst t1 k u) (subst t2 k u)
+  end.
+
+Inductive beta : term -> term -> Prop :=
+| beta_app1 : forall t1 t2 t3, beta t1 t2 -> beta (app t1 t3) (app t2 t3)
+| beta_app2 : forall t1 t2 t3, beta t1 t2 -> beta (app t3 t1) (app t3 t2)
+| beta_abs : forall t1 t2, beta t1 t2 -> beta (abs t1) (abs t2)
+| beta_redex : forall t1 t2, beta (app (abs t1) t2) (subst t1 0 t2).
+
+Inductive deep_flag := shallow | deep.
+Lemma deep_flag_eq_dec : forall (df1 df2 : deep_flag), { df1 = df2 } + { df1 <> df2 }.
+Proof.
+  intros [|] [|]; solve [left; reflexivity | right; discriminate].
+Defined.
+
+Inductive nfval :=
+| nvar : nat -> nfval
+| napp : nfval -> nfval_or_lam -> nfval
+
+with nfval_or_lam :=
+| nval : nfval -> nfval_or_lam
+| nlam : nfval_or_lam -> nfval_or_lam.
+
+Fixpoint read_nfval v :=
+  match v with
+  | nvar n => var n
+  | napp v1 v2 => app (read_nfval v1) (read_nfval_or_lam v2)
+  end
+
+with read_nfval_or_lam v :=
+  match v with
+  | nval v => read_nfval v
+  | nlam v => abs (read_nfval_or_lam v)
+  end.
+
+Inductive val : deep_flag -> Type :=
+| vals_nf : nfval -> val shallow
+| vals_abs : term -> val shallow
+| vald_nf : nfval_or_lam -> val deep.
+
+Definition read_val {df} (v : val df) :=
+  match v with
+  | vals_nf v => read_nfval v
+  | vals_abs t => abs t
+  | vald_nf v => read_nfval_or_lam v
+  end.
+
+Definition val_nf {df} v : val df :=
+  match df with
+  | shallow => vals_nf v
+  | deep => vald_nf (nval v)
+  end.
+
+Lemma read_val_nf :
+  forall df v, read_val (@val_nf df v) = read_nfval v.
+Proof.
+  intros [|] v; simpl; reflexivity.
+Qed.
+
+Inductive out t :=
+| out_ret : t -> out t
+| out_div : out t.
+
+Arguments out_ret {t} _.
+Arguments out_div {t}.
+
+Inductive ext : deep_flag -> Type :=
+| ext_term : forall df, term -> ext df
+| ext_app : forall df, out (val shallow) -> term -> ext df
+| ext_appnf : forall df, nfval -> out (val deep) -> ext df
+| extd_abs : out (val deep) -> ext deep.
+
+Arguments ext_term {df} _.
+Arguments ext_app {df} _ _.
+Arguments ext_appnf {df} _ _.
+
+Inductive red : forall df, ext df -> out (val df) -> Prop :=
+| red_var : forall df n, red df (ext_term (var n)) (out_ret (val_nf (nvar n))) (* Free variables reduce to themselves *)
+| red_abs_shallow : forall t, red shallow (ext_term (abs t)) (out_ret (vals_abs t)) (* Do not look under abstractions *)
+| red_abs_deep : forall t o1 o2,
+    red deep (ext_term t) o1 ->
+    red deep (extd_abs o1) o2 ->
+    red deep (ext_term (abs t)) o2
+| red_abs1_abort : red deep (extd_abs out_div) out_div
+| red_abs1 : forall v, red deep (extd_abs (out_ret (vald_nf v))) (out_ret (vald_nf (nlam v)))
+| red_app : forall df t1 o1 t2 o2,
+    red shallow (ext_term t1) o1 ->
+    red df (ext_app o1 t2) o2 ->
+    red df (ext_term (app t1 t2)) o2
+| red_app1_abort : forall df t2, red df (ext_app out_div t2) out_div
+| red_app1_nf : forall df v o1 t2 o2,
+    red deep (ext_term t2) o1 ->
+    red df (ext_appnf v o1) o2 ->
+    red df (ext_app (out_ret (vals_nf v)) t2) o2
+| red_app1_abs : forall df t1 t2 o,
+    red df (ext_term (subst t1 0 t2)) o ->
+    red df (ext_app (out_ret (vals_abs t1)) t2) o
+| red_appnf_abort : forall df v, red df (ext_appnf v out_div) out_div
+| red_appnf : forall df v1 v2, red df (ext_appnf v1 (out_ret (vald_nf v2))) (out_ret (val_nf (napp v1 v2))).
+
+CoInductive cored : forall df, ext df -> out (val df) -> Prop :=
+| cored_var : forall df n, cored df (ext_term (var n)) (out_ret (val_nf (nvar n))) (* Free variables reduce to themselves *)
+| cored_abs_shallow : forall t, cored shallow (ext_term (abs t)) (out_ret (vals_abs t)) (* Do not look under abstractions *)
+| cored_abs_deep : forall t o1 o2,
+    cored deep (ext_term t) o1 ->
+    cored deep (extd_abs o1) o2 ->
+    cored deep (ext_term (abs t)) o2
+| cored_abs1_abort : cored deep (extd_abs out_div) out_div
+| cored_abs1 : forall v, cored deep (extd_abs (out_ret (vald_nf v))) (out_ret (vald_nf (nlam v)))
+| cored_app : forall df t1 o1 t2 o2,
+    cored shallow (ext_term t1) o1 ->
+    cored df (ext_app o1 t2) o2 ->
+    cored df (ext_term (app t1 t2)) o2
+| cored_app1_abort : forall df t2, cored df (ext_app out_div t2) out_div
+| cored_app1_nf : forall df v o1 t2 o2,
+    cored deep (ext_term t2) o1 ->
+    cored df (ext_appnf v o1) o2 ->
+    cored df (ext_app (out_ret (vals_nf v)) t2) o2
+| cored_app1_abs : forall df t1 t2 o,
+    cored df (ext_term (subst t1 0 t2)) o ->
+    cored df (ext_app (out_ret (vals_abs t1)) t2) o
+| cored_appnf_abort : forall df v, cored df (ext_appnf v out_div) out_div
+| cored_appnf : forall df v1 v2, cored df (ext_appnf v1 (out_ret (vald_nf v2))) (out_ret (val_nf (napp v1 v2))).
+
+CoInductive infred {A : Type} (R : A -> A -> Prop) : A -> Prop :=
+| infred_step : forall x y, R x y -> infred R y -> infred R x.
+CoInductive costar {A : Type} (R : A -> A -> Prop) : A -> option A -> Prop :=
+| costar_refl : forall x, costar R x (Some x)
+| costar_step : forall x y z, R x y -> costar R y z -> costar R x z.
+CoInductive costarT {A : Type} (R : A -> A -> Prop) : A -> option A -> Prop :=
+| costarT_refl : forall x, costarT R x (Some x)
+| costarT_step : forall x y z, R x y -> costarT R y z -> costarT R x z
+| costarT_comp : forall w x y z, R w x -> costarT R x y -> (forall v, y = Some v -> costarT R v z) -> costarT R w z.
+Definition costarP {A : Type} (R : A -> A -> Prop) x y :=
+  exists H, H x y /\ forall x1 y1, H x1 y1 -> y1 = Some x1 \/ exists z, R x1 z /\ H z y1.
+Definition costarPT {A : Type} (R : A -> A -> Prop) x y :=
+  exists H, H x y /\ forall x1 y1, H x1 y1 -> y1 = Some x1 \/ (exists z, R x1 z /\ H z y1) \/ exists z1 z2, R x1 z1 /\ H z1 z2 /\ (forall v, z2 = Some v -> H v y1).
+
+Inductive costarZ_gen {A : Type} (R : A -> A -> Prop) (H : A -> option A -> Prop) : A -> option A -> Prop :=
+| costarZ_gen_refl : forall x, costarZ_gen R H x (Some x)
+| costarZ_gen_step : forall x y z, R x y -> H y z -> costarZ_gen R H x z
+| costarZ_gen_comp : forall x y z, costarZ_gen R H x y -> (forall w, y = Some w -> costarZ_gen R H w z) -> costarZ_gen R H x z.
+Definition costarZ {A : Type} (R : A -> A -> Prop) x y :=
+  exists H, H x y /\ forall x1 y1, H x1 y1 -> costarZ_gen R H x1 y1.
+Inductive costarW_gen {A : Type} (R : A -> A -> Prop) (H : A -> option A -> Prop) : A -> option A -> Prop :=
+| costarW_gen_refl : forall x, costarW_gen R H x (Some x)
+| costarW_gen_step : forall x y z, R x y -> H y z -> costarW_gen R H x z
+| costarW_gen_comp : forall x y z, costarW_gen R H x y -> (forall w, y = Some w -> H w z) -> costarW_gen R H x z.
+Definition costarW {A : Type} (R : A -> A -> Prop) x y :=
+  exists H, H x y /\ forall x1 y1, H x1 y1 -> costarW_gen R H x1 y1.
+
+Lemma costarP_costar :
+  forall A (R : A -> A -> Prop) x y, costarP R x y -> costar R x y.
+Proof.
+  intros A R. cofix IH. intros x y (H & H1 & H2).
+  apply H2 in H1. destruct H1 as [H1 | (z & HR & H1)].
+  - subst. constructor.
+  - econstructor; [eassumption|]. apply IH. exists H; split; assumption.
+Qed.
+
+Lemma costarPT_costarT :
+  forall A (R : A -> A -> Prop) x y, costarPT R x y -> costarT R x y.
+Proof.
+  intros A R. cofix IH. intros x y (H & H1 & H2).
+  apply H2 in H1. destruct H1 as [H1 | [(z & HR & H1) | (z1 & z2 & HR & H1a & H1b)]].
+  - subst. constructor.
+  - econstructor; [eassumption|]. apply IH. exists H; split; assumption.
+  - eapply costarT_comp; [eassumption| |].
+    + apply IH. exists H; split; eassumption.
+    + intros v ->. apply IH. exists H; split; [|eassumption]. apply H1b. reflexivity.
+Qed.
+
+Lemma costarT_comp1 :
+  forall A (R : A -> A -> Prop) x y z, costarT R x y -> (forall v, y = Some v -> costarT R v z) -> costarT R x z.
+Proof.
+  intros A R. cofix IH. intros x y z H1 H2. inversion H1; subst.
+  - apply H2. reflexivity.
+  - eapply costarT_step; [eassumption|]. eapply IH; eassumption.
+  - eapply costarT_comp; [eassumption|eassumption|].
+    intros v Hv; eapply IH.
+    + apply H3. assumption.
+    + assumption.
+Qed.
+
+Lemma costarT_costarP :
+  forall A (R : A -> A -> Prop) x y, costarT R x y -> costarP R x y.
+Proof.
+  intros A R x y H. exists (costarT R).
+  split; [assumption|]. intros x1 y1 H1. inversion H1; subst.
+  - left; reflexivity.
+  - right; eexists; split; eassumption.
+  - right; eexists; split; [eassumption|].
+    eapply costarT_comp1; eassumption.
+Qed.
+
+Lemma costarZ_gen_mono : forall A (R : A -> A -> Prop) (H1 H2 : A -> option A -> Prop) x y,
+    (forall x y, H1 x y -> H2 x y) -> costarZ_gen R H1 x y -> costarZ_gen R H2 x y.
+Proof.
+  intros A R H1 H2 x y H12 Hgen. induction Hgen.
+  - apply costarZ_gen_refl.
+  - eapply costarZ_gen_step; [eassumption|]. apply H12. assumption.
+  - eapply costarZ_gen_comp; [eassumption|]. eassumption.
+Qed.
+
+Lemma costarW_gen_mono : forall A (R : A -> A -> Prop) (H1 H2 : A -> option A -> Prop) x y,
+    (forall x y, H1 x y -> H2 x y) -> costarW_gen R H1 x y -> costarW_gen R H2 x y.
+Proof.
+  intros A R H1 H2 x y H12 Hgen. induction Hgen.
+  - apply costarW_gen_refl.
+  - eapply costarW_gen_step; [eassumption|]. apply H12. assumption.
+  - eapply costarW_gen_comp; [eassumption|]. intros w Hw. apply H12. apply H; assumption.
+Qed.
+
+Lemma costarZ_comp :
+  forall A (R : A -> A -> Prop) x y z, costarZ R x y -> (forall v, y = Some v -> costarZ R v z) -> costarZ R x z.
+Proof.
+  intros A R x y z H1 H2. destruct y as [y|].
+  - specialize (H2 y eq_refl). destruct H1 as (H1 & H1a & H1b). destruct H2 as (H2 & H2a & H2b).
+    exists (fun u v => H1 u v \/ H2 u v \/ exists w, H1 u (Some w) /\ H2 w v).
+    split.
+    + right. right. exists y. split; assumption.
+    + clear x y z H1a H2a. intros x z [Hxz | [Hxz | (y & Hxy & Hyz)]].
+      * eapply costarZ_gen_mono; [|apply H1b; assumption].
+        intros; tauto.
+      * eapply costarZ_gen_mono; [|apply H2b; assumption].
+        intros; tauto.
+      * eapply costarZ_gen_comp.
+        -- eapply costarZ_gen_mono; [|apply H1b; apply Hxy].
+           intros; tauto.
+        -- intros w [= <-]. eapply costarZ_gen_mono; [|apply H2b; apply Hyz].
+           intros; tauto.
+  - destruct H1 as (H1 & H1a & H1b). exists (fun u v => H1 u v \/ H1 u None).
+    split; [right; assumption|]. clear x z H1a H2.
+    intros x y [Hxy | Hxy].
+    + eapply costarZ_gen_mono; [|apply H1b; assumption].
+      intros; tauto.
+    + apply H1b in Hxy. remember None as z; revert Heqz; induction Hxy.
+      * discriminate.
+      * intros ->. eapply costarZ_gen_step; [eassumption|]. right. assumption.
+      * intros ->. eapply costarZ_gen_comp; [eapply costarZ_gen_mono; [|eassumption]; intros; tauto|].
+        intros; apply H0; [assumption | reflexivity].
+Qed.
+
+Lemma costarW_comp :
+  forall A (R : A -> A -> Prop) x y z, costarW R x y -> (forall v, y = Some v -> costarW R v z) -> costarW R x z.
+Proof.
+  intros A R x y z H1 H2. destruct y as [y|].
+  - specialize (H2 y eq_refl). destruct H1 as (H1 & H1a & H1b). destruct H2 as (H2 & H2a & H2b).
+    exists (fun u v => H1 u v \/ H2 u v \/ exists w, H1 u (Some w) /\ H2 w v).
+    split.
+    + right. right. exists y. split; assumption.
+    + clear x y z H1a H2a. intros x z [Hxz | [Hxz | (y & Hxy & Hyz)]].
+      * eapply costarW_gen_mono; [|apply H1b; assumption].
+        intros; tauto.
+      * eapply costarW_gen_mono; [|apply H2b; assumption].
+        intros; tauto.
+      * eapply costarW_gen_comp.
+        -- eapply costarW_gen_mono; [|apply H1b; apply Hxy].
+           intros; tauto.
+        -- intros w [= <-]. tauto.
+  - destruct H1 as (H1 & H1a & H1b). exists (fun u v => H1 u v \/ H1 u None).
+    split; [right; assumption|]. clear x z H1a H2.
+    intros x y [Hxy | Hxy].
+    + eapply costarW_gen_mono; [|apply H1b; assumption].
+      intros; tauto.
+    + apply H1b in Hxy. remember None as z; revert Heqz; induction Hxy.
+      * discriminate.
+      * intros ->. eapply costarW_gen_step; [eassumption|]. right. assumption.
+      * intros ->. eapply costarW_gen_comp; [eapply costarW_gen_mono; [|eassumption]; intros; tauto|].
+        intros. right. apply H. assumption.
+Qed.
+
+
+Lemma costarZ_costarP :
+  forall A (R : A -> A -> Prop) x y, costarZ R x y -> costarP R x y.
+Proof.
+  intros A R x y H. exists (costarZ R).
+  split; [assumption|]. clear x y H. intros x y H. destruct H as (H & H1 & H2).
+  apply H2 in H1. induction H1.
+  - left. reflexivity.
+  - right. exists y. split; [assumption|]. eexists; split; eassumption.
+  - destruct IHcostarZ_gen as [-> | (w & Hw1 & Hw2)].
+    + apply H3. reflexivity.
+    + right. exists w; split; [assumption|].
+      eapply costarZ_comp; [eassumption|].
+      intros v ->. specialize (H0 v eq_refl).
+      exists (fun u v => H u v \/ costarZ_gen R H u v).
+      split; [right; assumption|].
+      intros s t [Hst | Hst].
+      * eapply costarZ_gen_mono; [|apply H2; assumption]; intros; tauto.
+      * eapply costarZ_gen_mono; [|apply Hst; assumption]; intros; tauto.
+Qed.
+
+Lemma costarW_costarP :
+  forall A (R : A -> A -> Prop) x y, costarW R x y -> costarP R x y.
+Proof.
+  intros A R x y H. exists (costarW R).
+  split; [assumption|]. clear x y H. intros x y H. destruct H as (H & H1 & H2).
+  apply H2 in H1. induction H1.
+  - left. reflexivity.
+  - right. exists y. split; [assumption|]. eexists; split; eassumption.
+  - destruct IHcostarW_gen as [-> | (w & Hw1 & Hw2)].
+Abort. (*
+    + apply H3. reflexivity.
+    + right. exists w; split; [assumption|].
+      eapply costarW_comp; [eassumption|].
+      intros v ->. specialize (H0 v eq_refl).
+      exists (fun u v => H u v \/ costarZ_gen R H u v).
+      split; [right; assumption|].
+      intros s t [Hst | Hst].
+      * eapply costarZ_gen_mono; [|apply H2; assumption]; intros; tauto.
+      * eapply costarZ_gen_mono; [|apply Hst; assumption]; intros; tauto.
+Qed.
+*)
+
+
+Lemma costarPT_costarP :
+  forall A (R : A -> A -> Prop) x y, costarPT R x y -> costarP R x y.
+Proof.
+  intros A R x y H. exists (costarPT R). split; [assumption|]. clear x y H.
+  intros x y (H & H1 & H2). apply H2 in H1. destruct H1 as [H1 | [H1 | H1]].
+  - left; assumption.
+  - right. destruct H1 as (z & Hz1 & Hz2). exists z. split; [assumption|]. exists H. split; assumption.
+  - admit.
+Abort.
+
+Definition read_out {df} (o : out (val df)) := match o with out_div => None | out_ret v => Some (read_val v) end.
+Definition read_ext {df} (e : ext df) :=
+  match e with
+  | ext_term t => Some t
+  | ext_app o t2 => match read_out o with Some t1 => Some (app t1 t2) | None => None end
+  | ext_appnf v1 o => match read_out o with Some t2 => Some (app (read_nfval v1) t2) | None => None end
+  | extd_abs o => match read_out o with Some t => Some (abs t) | None => None end
+  end.
+
+Require Import Star.
+Require Import Coq.Logic.Eqdep_dec.
+
+Lemma red_star_beta :
+  forall df e o, red df e o -> forall t1 t2, read_ext e = Some t1 -> read_out o = Some t2 -> star beta t1 t2.
+Proof.
+  intros df e o H. induction H; intros u1 u2 Hu1 Hu2; simpl in *.
+  - rewrite read_val_nf in Hu2; simpl in Hu2.
+    injection Hu1; injection Hu2; intros; subst. constructor.
+  - injection Hu1; injection Hu2; intros; subst. constructor.
+  - destruct o1.
+    + simpl in *. eapply star_compose.
+      * injection Hu1; intros; subst. eapply star_map_impl with (RA := beta); [intros; constructor; assumption|].
+        apply IHred1; reflexivity.
+      * apply IHred2; [reflexivity|assumption].
+    + inversion H0; subst.
+      apply inj_pair2_eq_dec in H1; [|apply deep_flag_eq_dec].
+      subst; simpl in *; congruence.
+  - congruence.
+  - injection Hu1; injection Hu2; intros; subst. constructor.
+  - destruct o1.
+    + simpl in *. eapply star_compose.
+      * injection Hu1; intros; subst.
+        eapply star_map_impl with (f := fun t => app t t2) (RA := beta); [intros; constructor; assumption|].
+        eapply IHred1; reflexivity.
+      * apply IHred2; [reflexivity|assumption].
+    + inversion H0; subst.
+      apply inj_pair2_eq_dec in H4; [|apply deep_flag_eq_dec].
+      subst; simpl in *; congruence.
+  - congruence.
+  - destruct o1.
+    + simpl in *. eapply star_compose.
+      * injection Hu1; intros; subst.
+        eapply star_map_impl with (f := fun t => app _ t) (RA := beta); [intros; constructor; assumption|].
+        eapply IHred1; reflexivity.
+      * apply IHred2; [reflexivity|assumption].
+    + inversion H0; subst.
+      apply inj_pair2_eq_dec in H4; [|apply deep_flag_eq_dec].
+      subst; simpl in *; congruence.
+  - injection Hu1; intros; subst.
+    econstructor; [apply beta_redex|].
+    apply IHred; [reflexivity|assumption].
+  - congruence.
+  - injection Hu1; injection Hu2; intros; subst.
+    rewrite read_val_nf. simpl. constructor.
+Qed.
+
+Lemma infred_map_impl :
+  forall (A B : Type) (RA : A -> A -> Prop) (RB : B -> B -> Prop) (f : A -> B),
+    (forall x y : A, RA x y -> RB (f x) (f y)) -> forall x : A, infred RA x -> infred RB (f x).
+Proof.
+  intros A B RA RB f H. cofix IH. intros x Hx. inversion Hx; subst.
+  econstructor; [apply H; eassumption|].
+  apply IH. assumption.
+Qed.
+
+Lemma costar_map_impl :
+  forall (A B : Type) (RA : A -> A -> Prop) (RB : B -> B -> Prop) (f : A -> B),
+    (forall x y : A, RA x y -> RB (f x) (f y)) ->
+    forall x y, costar RA x y -> costar RB (f x) (match y with None => None | Some y => Some (f y) end).
+Proof.
+  intros A B RA RB f H. cofix IH. intros x y Hx. inversion Hx; subst.
+  - constructor.
+  - econstructor; [apply H; eassumption|].
+    apply IH. assumption.
+Qed.
+
+Lemma costarT_map_impl :
+  forall (A B : Type) (RA : A -> A -> Prop) (RB : B -> B -> Prop) (f : A -> B),
+    (forall x y : A, RA x y -> RB (f x) (f y)) ->
+    forall x y, costarT RA x y -> costarT RB (f x) (match y with None => None | Some y => Some (f y) end).
+Proof.
+  intros A B RA RB f H. cofix IH. intros x y Hx. inversion Hx; subst.
+  - constructor.
+  - econstructor; [apply H; eassumption|].
+    apply IH. assumption.
+  - econstructor; [apply H; eassumption| |].
+    + apply IH. eassumption.
+    + destruct y0 as [y1|]; intros v; [|discriminate]; intros [= <-].
+      apply IH. apply H2. reflexivity.
+Defined.
+Print costarT_map_impl.
+Eval cbv in costarT_map_impl.
+
+Lemma costar_compose :
+  forall (A : Type) (R : A -> A -> Prop) x y z,
+    costar R x y -> (forall w, y = Some w -> costar R w z) -> costar R x z.
+Proof.
+  intros A R. cofix IH. intros x y z H1 H2. inversion H1; subst.
+  - apply H2. reflexivity.
+  - econstructor; [eassumption|].
+    eapply IH; eassumption.
+Defined.
+
+Ltac unexistT :=
+  repeat match goal with
+           [ H : @existT deep_flag _ _ _ = @existT deep_flag _ _ _ |- _ ] =>
+           apply inj_pair2_eq_dec in H; [|apply deep_flag_eq_dec]
+         end.
+
+Definition option_map {A B : Type} (f : A -> B) (x : option A) := match x with Some x => Some (f x) | None => None end.
+Lemma option_map_id : forall (A : Type) (x : option A), option_map id x = x.
+Proof.
+  intros A [x|]; reflexivity.
+Qed.
+
+Definition respectful {A : Type} (R : A -> A -> Prop) (f : A -> A) := forall x y, R x y -> R (f x) (f y).
+
+(*
+Lemma red_div_beta :
+  forall t df e o, cored df e o -> read_ext e = Some t -> costarPT (fun x y => beta x y \/ x = y) t (read_out o).
+Proof.
+  intros t df e o H Ht.
+  exists (fun x y => exists df e o f, cored df e o /\ option_map f (read_ext e) = Some x /\ y = option_map f (read_out o) /\ respectful beta f).
+  split; [exists df; exists e; exists o; exists id; split; [assumption|split; rewrite option_map_id; [assumption|split; [reflexivity|intros x y Hxy; assumption]]]|].
+  clear t df e o H Ht. intros t y (df & e & o & f & H & Ht & -> & Hf);
+  inversion H; subst; simpl in *; unexistT; subst; simpl in *; try congruence; injection Ht; intros; subst.
+  - left. rewrite read_val_nf. reflexivity.
+  - left. reflexivity.
+  - right. right.
+    eexists. eexists. split; [right; reflexivity|]. split.
+    + eexists. eexists. eexists. exists (fun t1 => f (abs t1)).
+      split; [exact H4|]. simpl. split; [reflexivity|]. split; [reflexivity|]. intros x y Hxy. apply Hf. apply beta_abs. assumption.
+    + intros v Hv. destruct o1; simpl in Hv; [|discriminate]. injection Hv; intros; subst.
+      eexists. eexists. eexists. exists f.
+      split; [exact H6|]. split; [reflexivity|]. split; [reflexivity|]. assumption.
+  - left. reflexivity.
+  - right. right.
+    eexists. eexists. split; [right; reflexivity|]. split.
+    + eexists. eexists. eexists. exists (fun t3 => f (app t3 t2)).
+      split; [exact H3|]. simpl. split; [reflexivity|]. split; [reflexivity|]. intros x y Hxy. apply Hf. apply beta_app1. assumption.
+    + intros v Hv. destruct o1; simpl in Hv; [|discriminate]. injection Hv; intros; subst.
+      eexists. eexists. eexists. exists f.
+      split; [exact H4|]. simpl. split; [reflexivity|]. split; [reflexivity|]. assumption.
+  - right. right.
+    eexists. eexists. split; [right; reflexivity|]. split.
+    + eexists. eexists. eexists. exists (fun t3 => f (app (read_nfval v) t3)).
+      split; [exact H3|]. simpl. split; [reflexivity|]. split; [reflexivity|]. intros x y Hxy. apply Hf. apply beta_app2. assumption.
+    + intros w Hw. destruct o1; simpl in Hw; [|discriminate]. injection Hw; intros; subst.
+      eexists. eexists. eexists. exists f.
+      split; [exact H4|]. simpl. split; [reflexivity|]. split; [reflexivity|]. assumption.
+  - right. left.
+    exists (f (subst t1 0 t2)). split; [left; apply Hf; apply beta_redex|].
+    eexists. eexists. eexists. exists f.
+    split; [exact H3|]. simpl. split; [reflexivity|]. split; [reflexivity|]. assumption.
+  - left. rewrite read_val_nf. reflexivity.
+Qed.
+ *)
+
+Fixpoint size t :=
+  match t with
+  | var n => 0
+  | abs t => S (size t)
+  | app t1 t2 => S (size t1 + size t2)
+  end.
+
+Definition read_ext_with_size {df} (e : ext df) :=
+  match e with
+  | ext_term t => Some (t, 2 * size t)
+  | ext_app o t2 => match read_out o with Some t1 => Some (app t1 t2, 2 * size t2 + 1) | None => None end
+  | ext_appnf v1 o => match read_out o with Some t2 => Some (app (read_nfval v1) t2, 0) | None => None end
+  | extd_abs o => match read_out o with Some t => Some (abs t, 0) | None => None end
+  end.
+Definition read_out_with_size {df} (o : out (val df)) := match o with out_div => None | out_ret v => Some (read_val v, 0) end.
+
+Definition fst_map {A B C : Type} (f : A -> B) : (A * C) -> (B * C) := fun x => (f (fst x), snd x).
+Lemma option_map_fst_id :
+  forall (A B : Type) (x : option (A * B)), option_map (fst_map id) x = x.
+Proof.
+  destruct x as [[x y]|]; simpl; reflexivity.
+Qed.
+
+Definition weaken {A : Type} (x y : A * nat) := fst x = fst y /\ snd y <= snd x.
+Definition weakenO {A : Type} (x y : option (A * nat)) := match x, y with None, None => True | Some x, Some y => weaken x y | _, _ => False end.
+
+Lemma weaken_refl : forall (A : Type) (x : A * nat), weaken x x.
+Proof.
+  intros A [x y]. unfold weaken. simpl. split; reflexivity.
+Qed.
+
+Lemma weakenO_refl : forall (A : Type) (x : option (A * nat)), weakenO x x.
+Proof.
+  intros A [x|]; unfold weakenO; simpl.
+  - apply weaken_refl.
+  - tauto.
+Qed.
+
+Definition stepped {A : Type} (R : A -> A -> Prop) x y := R (fst x) (fst y) \/ (fst x = fst y /\ snd y < snd x).
+
+Definition costarPTn {A : Type} (R : A -> A -> Prop) x y :=
+  exists H, H x y /\ forall x1 y1, H x1 y1 ->
+                        weakenO (Some x1) y1 \/
+                        (exists z1, stepped R x1 z1 /\ H z1 y1) \/
+                        (exists z1 z2, stepped R x1 z1 /\ H z1 z2 /\ (forall v, z2 = Some v -> H v y1)).
+
+Lemma costarPTn_destruct :
+  forall (A : Type) (R : A -> A -> Prop) x y,
+    costarPTn R x y -> weakenO (Some x) y \/
+                      (exists z, stepped R x z /\ costarPTn R z y) \/
+                      (exists z1 z2, stepped R x z1 /\ costarPTn R z1 z2 /\ (forall v, z2 = Some v -> costarPTn R v y)).
+Proof.
+  intros A R x y (H & H1 & H2).
+  apply H2 in H1. destruct H1 as [H1 | [(z & Hz1 & Hz2) | (z1 & z2 & Hz1 & Hz2 & Hz3)]].
+  - left. assumption.
+  - right. left. exists z. split; [assumption|]. exists H; split; assumption.
+  - right. right. exists z1. exists z2. split; [assumption|]. split.
+    + exists H; split; assumption.
+    + intros v ->. exists H; split; [|assumption]. apply Hz3. reflexivity.
+Qed.
+
+Lemma weaken_trans :
+  forall (A : Type) (x y z : A * nat), weaken x y -> weaken y z -> weaken x z.
+Proof.
+  intros A [x1 x2] [y1 y2] [z1 z2]; unfold weaken; simpl.
+  intros [? ?] [? ?]; split; [congruence|lia].
+Qed.
+
+Lemma stepped_weaken :
+  forall (A : Type) (R : A -> A -> Prop) x y z, weaken x y -> stepped R y z -> stepped R x z.
+Proof.
+  intros A R [x1 x2] [y1 y2] [z1 z2] [H1 H2] [H3 | [H3 H4]]; simpl in *; subst.
+  - left; simpl; assumption.
+  - right; simpl; split; [reflexivity|lia].
+Qed.
+
+Lemma costarPTn_comp :
+  forall (A : Type) (R : A -> A -> Prop) x y z, costarPTn R x y -> (forall v, y = Some v -> costarPTn R v z) -> costarPTn R x z.
+Proof.
+  intros A R x y z H1 H2. exists (fun x1 y1 => costarPTn R x1 y1 \/ exists w, costarPTn R x1 w /\ (forall v, w = Some v -> costarPTn R v y1)).
+  split.
+  - right. exists y. split; assumption.
+  - clear x y z H1 H2. intros x z [Hxz | (y & Hxy & Hyz)].
+    + apply costarPTn_destruct in Hxz. destruct Hxz as [Hxz | [(z1 & Hz1 & Hz2) | (z1 & z2 & Hz1 & Hz2 & Hz3)]].
+      * left. assumption.
+      * right. left. exists z1. split; tauto.
+      * right. right. exists z1. exists z2. split; [assumption|]. split; [tauto|]. intros v Hv; left; apply Hz3; assumption.
+    + apply costarPTn_destruct in Hxy. destruct Hxy as [Hxy | [(z1 & Hz1 & Hz2) | (z1 & z2 & Hz1 & Hz2 & Hz3)]].
+      * destruct y as [y|]; simpl in *; [|tauto].
+        specialize (Hyz y eq_refl).
+        apply costarPTn_destruct in Hyz. destruct Hyz as [Hyz | [(z1 & Hz1 & Hz2) | (z1 & z2 & Hz1 & Hz2 & Hz3)]].
+        -- destruct z as [z|]; simpl in *; [|tauto].
+           left. eapply weaken_trans; eassumption.
+        -- right. left. exists z1. split; [eapply stepped_weaken; eassumption|].
+           left; assumption.
+        -- right. right. exists z1. exists z2. split; [eapply stepped_weaken; eassumption|].
+           split; [left; assumption|]. intros; left; apply Hz3; assumption.
+      * right. left. exists z1. split; [assumption|].
+        right. exists y. split; assumption.
+      * right. right. exists z1. exists z2. split; [assumption|].
+        split.
+        -- left; assumption.
+        -- intros v ->. right. exists y. split; [apply Hz3; reflexivity|].
+           intros w ->. apply Hyz. reflexivity.
+Qed.
+
+
+Lemma costarPTn_costarP :
+  forall (A : Type) (R : A -> A -> Prop) x y, costarPTn R x y -> costarP R (fst x) (option_map fst y).
+Proof.
+  intros A R x y H. exists (fun u v => exists n m, costarPTn R (u, n) (option_map (fun v => (v, m)) v)).
+  split.
+  - exists (snd x). exists (match y with Some y => snd y | None => 0 end).
+    destruct x as [x1 x2]. destruct y as [[y1 y2]|]; simpl; assumption.
+  - clear x y H. intros x y (n & m & H).
+    revert x y m H; induction n as [n Hn] using lt_wf_ind; intros x y m H.
+    apply costarPTn_destruct in H. destruct H as [H | [(z & Hz1 & Hz2) | (z1 & z2 & Hz1 & Hz2 & Hz3)]].
+    + destruct y as [y|]; simpl in H; [|tauto].
+      unfold weaken in H; simpl in H. left. destruct H; congruence.
+    + destruct Hz1 as [Hz1 | Hz1]; simpl in Hz1.
+      * right. exists (fst z). split; [assumption|].
+        exists (snd z). exists m. destruct z; assumption.
+      * destruct Hz1 as [-> Hz1]. destruct z as [z1 z2]; simpl in *.
+        eapply Hn; [|eassumption]. assumption.
+    + destruct Hz1 as [Hz1 | Hz1]; simpl in Hz1.
+      * right. exists (fst z1). split; [assumption|].
+        exists (snd z1). exists m. eapply costarPTn_comp; [destruct z1; simpl in *; eassumption|].
+        eassumption.
+      * destruct Hz1 as [-> Hz1]. destruct z1 as [z3 z4]; simpl in *.
+        eapply Hn; [exact Hz1|].
+        eapply costarPTn_comp; eassumption.
+Qed.
+
+Lemma red_div_beta_aux :
+  forall t df e o, cored df e o -> read_ext_with_size e = Some t ->
+              costarPTn beta t (read_out_with_size o).
+Proof.
+  intros t df e o H Ht.
+  exists (fun x y => exists df e o f,
+         cored df e o /\
+         option_map f (read_ext_with_size e) = Some x /\
+         y = option_map f (read_out_with_size o) /\
+         respectful (stepped beta) f /\ respectful weaken f).
+  split.
+  {
+    exists df. exists e. exists o. exists id. splits 5.
+    - assumption.
+    - rewrite option_map_id. assumption.
+    - rewrite option_map_id. reflexivity.
+    - intros x y Hxy. exact Hxy.
+    - intros x y Hxy. exact Hxy.
+  }
+  clear t df e o H Ht. intros x y (df & e & o & f & H & Hx & -> & Hf).
+  inversion H; subst; simpl in *; unexistT; subst; simpl in *; try congruence; simpl in Hx; injection Hx as Hx; subst x.
+  - rewrite read_val_nf in *; simpl in *.
+    left. apply Hf. unfold weaken. split; simpl; [reflexivity|lia].
+  - left. apply Hf. unfold weaken. split; simpl; [reflexivity|lia].
+  - right; right.
+    simpl.
+    exists (f (abs t, 2 * size t)).
+    exists (option_map (fun t1 => f (abs (fst t1), snd t1)) (read_out_with_size o1)).
+    splits 3.
+    + apply Hf. right. simpl. split; [reflexivity|]. simpl. lia.
+    + eexists. eexists. eexists. exists (fun t1 => f (abs (fst t1), snd t1)).
+      split; [exact H4|]. simpl. split; [reflexivity|]. split; [reflexivity|].
+      split; intros x y Hxy; apply Hf.
+      * destruct Hxy as [Hxy | Hxy]; [left; simpl; constructor; assumption|right; simpl; split; [f_equal|]; tauto].
+      * unfold weaken in *. simpl. split; [f_equal|]; tauto.
+    + intros w Hw. destruct o1; simpl in Hw; [|discriminate]. injection Hw; intros; subst.
+      eexists. eexists. eexists. exists f.
+      split; [exact H6|]. simpl. split; [reflexivity|].
+      split; [reflexivity|]. apply Hf.
+  - left. apply Hf. apply weaken_refl.
+  - right. right.
+    exists (f (app t1 t2, 2 * size t1 + 2 * size t2 + 1)).
+    exists (option_map (fun t3 => f (app (fst t3) t2, snd t3 + 2 * size t2 + 1)) (read_out_with_size o1)).
+    splits 3.
+    + apply Hf. right. simpl. split; [reflexivity|lia].
+    + eexists. eexists. eexists. exists (fun t3 => f (app (fst t3) t2, snd t3 + 2 * size t2 + 1)).
+      split; [exact H3|]. simpl. split; [reflexivity|].
+      split; [reflexivity|].
+      split; intros x y Hxy; apply Hf.
+      * destruct Hxy as [Hxy | Hxy]; [left; simpl; constructor; assumption|right; simpl; split; [f_equal; tauto|lia]].
+      * unfold weaken in *. simpl. split; [f_equal; tauto|lia].
+    + intros v Hv. destruct o1; simpl in Hv; [|discriminate]. injection Hv; intros; subst.
+      eexists. eexists. eexists. exists f.
+      split; [exact H4|]. simpl. split; [reflexivity|]. split; [reflexivity|]. assumption.
+  - right. right.
+    exists (f (app (read_nfval v) t2, 2 * size t2)).
+    exists (option_map (fun t3 => f (app (read_nfval v) (fst t3), snd t3)) (read_out_with_size o1)).
+    splits 3.
+    + apply Hf. right. simpl. split; [reflexivity|lia].
+    + eexists. eexists. eexists. exists (fun t3 => f (app (read_nfval v) (fst t3), snd t3)).
+      split; [exact H3|]. simpl. split; [reflexivity|]. split; [reflexivity|].
+      split; intros x y Hxy; apply Hf.
+      * destruct Hxy as [Hxy | Hxy]; [left; simpl; constructor; assumption|right; simpl; split; [f_equal|]; tauto].
+      * unfold weaken in *. simpl. split; [f_equal|]; tauto.
+    + intros w Hw. destruct o1; simpl in Hw; [|discriminate]. injection Hw; intros; subst.
+      eexists. eexists. eexists. exists f.
+      split; [exact H4|]. simpl. split; [reflexivity|]. split; [reflexivity|]. assumption.
+  - right. left.
+    exists (f (subst t1 0 t2, 2 * size (subst t1 0 t2))).
+    split; [apply Hf; left; apply beta_redex|].
+    eexists. eexists. eexists. exists f.
+    split; [exact H3|]. simpl. split; [reflexivity|]. split; [reflexivity|]. assumption.
+  - left. rewrite read_val_nf. apply weaken_refl.
+Qed.
+
+Lemma read_ext_with_size_read_ext :
+  forall df (e : ext df), read_ext e = option_map fst (read_ext_with_size e).
+Proof.
+  intros. destruct e; simpl; try destruct read_out; simpl; reflexivity.
+Qed.
+
+Lemma read_out_with_size_read_out :
+  forall df (o : out (val df)), read_out o = option_map fst (read_out_with_size o).
+Proof.
+  intros. destruct o; simpl; reflexivity.
+Qed.
+
+Lemma red_div_beta :
+  forall t df e o, cored df e o -> read_ext e = Some t -> costar beta t (read_out o).
+Proof.
+  intros t df e o Hred He. apply costarP_costar.
+  rewrite read_ext_with_size_read_ext in He.
+  destruct read_ext_with_size as [t1|] eqn:Heqre; simpl in *; [|congruence].
+  injection He as He; subst.
+  rewrite read_out_with_size_read_out.
+  apply costarPTn_costarP. eapply red_div_beta_aux; eassumption.
+Qed.
+
+(*
+Require Import Coq.Arith.Wf_nat.
+Lemma red_div_beta2 :
+  forall t df e o, cored df e o -> read_ext e = Some t ->
+              costarZ beta t (read_out o).
+Proof.
+  intros t df e o H Ht.
+  exists (fun x y => exists df e o f, cored df e o /\ option_map f (read_ext e) = Some x /\
+                         y = option_map f (read_out o) /\ respectful beta f).
+  split.
+  {
+    exists df; exists e; exists o; exists id. splits 4.
+    - assumption.
+    - rewrite option_map_id. assumption.
+    - rewrite option_map_id. reflexivity.
+    - intros x y Hxy. exact Hxy.
+  }
+  clear t df e o H Ht. intros x y (df & e & o & f & H & Hx & -> & Hf).
+  rewrite read_ext_with_size_read_ext in Hx.
+  destruct (read_ext_with_size e) as [[re n]|] eqn:Heqre; simpl in *; [|congruence]. simpl in Hx; injection Hx as Hx; subst x.
+  revert df re e o f H Hf Heqre. induction n as [n IHn] using lt_wf_ind. intros df re e o f H Hf Heqre.
+  inversion H; subst; simpl in *; unexistT; subst; simpl in *; try congruence; injection Heqre; intros; subst.
+  - rewrite read_val_nf. apply costarZ_gen_refl.
+  - apply costarZ_gen_refl.
+  - eapply costarZ_gen_comp.
+    + eapply IHn with (f := fun t1 => f (abs t1)); [|exact H4| |reflexivity]; [lia|].
+      intros x y Hxy. apply Hf. apply beta_abs. assumption.
+    + intros w Hw. destruct o1; simpl in Hw; [|discriminate]. injection Hw; intros; subst.
+      eapply IHn with (f := f); [|exact H6|assumption|reflexivity]. simpl. lia.
+      split; [exact H6|]. split; [reflexivity|]. split; [reflexivity|]. assumption.
+  - left. reflexivity.
+  - right. right.
+    eexists. eexists. split; [right; reflexivity|]. split.
+    + eexists. eexists. eexists. exists (fun t3 => f (app t3 t2)).
+      split; [exact H3|]. simpl. split; [reflexivity|]. split; [reflexivity|]. intros x y Hxy. apply Hf. apply beta_app1. assumption.
+    + intros v Hv. destruct o1; simpl in Hv; [|discriminate]. injection Hv; intros; subst.
+      eexists. eexists. eexists. exists f.
+      split; [exact H4|]. simpl. split; [reflexivity|]. split; [reflexivity|]. assumption.
+  - right. right.
+    eexists. eexists. split; [right; reflexivity|]. split.
+    + eexists. eexists. eexists. exists (fun t3 => f (app (read_nfval v) t3)).
+      split; [exact H3|]. simpl. split; [reflexivity|]. split; [reflexivity|]. intros x y Hxy. apply Hf. apply beta_app2. assumption.
+    + intros w Hw. destruct o1; simpl in Hw; [|discriminate]. injection Hw; intros; subst.
+      eexists. eexists. eexists. exists f.
+      split; [exact H4|]. simpl. split; [reflexivity|]. split; [reflexivity|]. assumption.
+  - right. left.
+    exists (f (subst t1 0 t2)). split; [left; apply Hf; apply beta_redex|].
+    eexists. eexists. eexists. exists f.
+    split; [exact H3|]. simpl. split; [reflexivity|]. split; [reflexivity|]. assumption.
+  - left. rewrite read_val_nf. reflexivity.
+Qed.
+*)
+
+(*
+  cofix IH. intros t df e o H Ht;
+              inversion H; subst; simpl in *; unexistT; subst; simpl in *; try congruence; injection Ht; intros; subst.
+  - rewrite read_val_nf; simpl. constructor.
+  - constructor.
+  - eapply costarT_comp with (y := match read_out o1 with | Some y => Some (abs y) | None => None end); [right; reflexivity| |].
+    + eapply costarT_map_impl; [|eapply IH; [exact H4|reflexivity]].
+      intros u1 u2 [Hu|Hu]; [left; constructor; assumption|right; congruence].
+    + intros w. destruct o1; simpl; [|discriminate]; intros [= <-].
+      eapply IH; [exact H6|reflexivity].
+  - constructor.
+  - admit.
+  - admit.
+  - eapply costarT_step; [left; apply beta_redex|].
+    eapply IH; [apply H3|]. reflexivity.
+  - rewrite read_val_nf; simpl. constructor.
+Qed.
+
+  - inversion H5; subst. injection Ht; intros; subst.
+    eapply infred_map_impl with (RA := beta) (f := abs); [intros; constructor; assumption|].
+    admit.
+  - 
+  - admit.
+
+  - apply inj_pair2_eq_dec in H1; [|apply deep_flag_eq_dec].
+    apply inj_pair2_eq_dec in H3; [|apply deep_flag_eq_dec].
+    subst. simpl in *. congruence.
+  - apply inj_pair2_eq_dec in H3; [|apply deep_flag_eq_dec].
+    subst. simpl in *. congruence.
+  - apply inj_pair2_eq_dec in H0; [|apply deep_flag_eq_dec].
+    apply inj_pair2_eq_dec in H1; [|apply deep_flag_eq_dec].
+    subst. simpl in *. congruence.
+  - apply inj_pair2_eq_dec in H2; [|apply deep_flag_eq_dec].
+    subst. simpl in *. congruence.
+  - apply inj_pair2_eq_dec in H0; [|apply deep_flag_eq_dec].
+    apply inj_pair2_eq_dec in H1; [|apply deep_flag_eq_dec].
+    subst. simpl in *. congruence.
+  - apply inj_pair2_eq_dec in H0; [|apply deep_flag_eq_dec].
+    apply inj_pair2_eq_dec in H2; [|apply deep_flag_eq_dec].
+    subst. simpl in *. congruence.
+  - apply inj_pair2_eq_dec in H2; [|apply deep_flag_eq_dec].
+    subst. simpl in *. congruence.
+  - 
+
+
+  cofix IH. intros df e H. inversion H; subst; intros u Hu; simpl in *.
+  - apply inj_pair2_eq_dec in H1; [|apply deep_flag_eq_dec].
+    apply inj_pair2_eq_dec in H3; [|apply deep_flag_eq_dec].
+    subst. injection Hu; intros; subst.
+    eapply infred_map_impl with (RA := beta) (f := abs); [intros; constructor; assumption|].
+    destruct o1.
+    + admit.
+    + eapply IH; [exact H4|]. reflexivity.
+  - congruence.
+  - admit.
+  - congruence.
+  - admit.
+  - admit.
+  - congruence.
+Qed.
+
+    rewrite read_val_nf in Hu2; simpl in Hu2.
+    injection Hu1; injection Hu2; intros; subst. constructor.
+  - injection Hu1; injection Hu2; intros; subst. constructor.
+  - destruct o1.
+    + simpl in *. eapply star_compose.
+      * injection Hu1; intros; subst. eapply star_map_impl with (RA := beta); [intros; constructor; assumption|].
+        apply IHred1; reflexivity.
+      * apply IHred2; [reflexivity|assumption].
+    + inversion H0; subst.
+      apply inj_pair2_eq_dec in H1; [|apply deep_flag_eq_dec].
+      subst; simpl in *; congruence.
+  - congruence.
+  - injection Hu1; injection Hu2; intros; subst. constructor.
+  - destruct o1.
+    + simpl in *. eapply star_compose.
+      * injection Hu1; intros; subst.
+        eapply star_map_impl with (f := fun t => app t t2) (RA := beta); [intros; constructor; assumption|].
+        eapply IHred1; reflexivity.
+      * apply IHred2; [reflexivity|assumption].
+    + inversion H0; subst.
+      apply inj_pair2_eq_dec in H4; [|apply deep_flag_eq_dec].
+      subst; simpl in *; congruence.
+  - congruence.
+  - destruct o1.
+    + simpl in *. eapply star_compose.
+      * injection Hu1; intros; subst.
+        eapply star_map_impl with (f := fun t => app _ t) (RA := beta); [intros; constructor; assumption|].
+        eapply IHred1; reflexivity.
+      * apply IHred2; [reflexivity|assumption].
+    + inversion H0; subst.
+      apply inj_pair2_eq_dec in H4; [|apply deep_flag_eq_dec].
+      subst; simpl in *; congruence.
+  - injection Hu1; intros; subst.
+    econstructor; [apply beta_redex|].
+    apply IHred; [reflexivity|assumption].
+  - congruence.
+  - injection Hu1; injection Hu2; intros; subst.
+    rewrite read_val_nf. simpl. constructor.
+Qed.
+*)
+
+
+
+
+
+
+
+
+
+
+
+
+
+
+
+
+
+(* STerms *)
+
+Inductive sterm :=
+| sbvar : nat -> sterm
+| sevar : nat -> sterm
+| sfvar : freevar -> sterm
+| slam : sterm -> sterm
+| sapp : sterm -> sterm -> sterm.
+
+Inductive sitem :=
+| sitem1 : sterm -> sitem
+| sitem2 : sterm -> sterm -> sitem.
+
+Definition readitem si :=
+  match si with
+  | sitem1 t => t
+  | sitem2 t1 t2 => t1
+  end.
+
+Fixpoint ssubstb k u t :=
+  match t with
+  | sbvar n => if Nat.eq_dec n k then u else sbvar n
+  | sevar n => sevar n
+  | sfvar x => sfvar x
+  | slam t => slam (ssubstb (S k) u t)
+  | sapp t1 t2 => sapp (ssubstb k u t1) (ssubstb k u t2)
+  end.
+
+Fixpoint sshifte k off t :=
+  match t with
+  | sbvar n => sbvar n
+  | sevar n => if le_lt_dec k n then sevar (off + n) else sevar n
+  | sfvar x => sfvar x
+  | slam t => slam (sshifte k off t)
+  | sapp t1 t2 => sapp (sshifte k off t1) (sshifte k off t2)
+  end.
+
+Definition sishifte k off si :=
+  match si with
+  | sitem1 t => sitem1 (sshifte k off t)
+  | sitem2 t1 t2 => sitem2 (sshifte k off t1) (sshifte k off t2)
+  end.
+
+Fixpoint seshifte k off e :=
+  match e with
+  | nil => nil
+  | si :: e => sishifte k off si :: seshifte k off e
+  end.
+
+Inductive sterm_red : list sterm -> sterm -> sterm -> list sterm -> Prop :=
+| sterm_red_var : forall env n t, nth_error env n = Some t -> sterm_red env (sevar n) t nil
+| sterm_red_app1 : forall env t1 t2 t3 e, sterm_red env t1 t2 e -> sterm_red env (sapp t1 t3) (sapp t2 t3) e
+| sterm_red_app2 : forall env t1 t2 t3 e, sterm_red env t1 t2 e -> sterm_red env (sapp t3 t1) (sapp t3 t2) e
+| sterm_red_lam : forall env t1 t2 e, sterm_red env t1 t2 e -> sterm_red env (slam t1) (slam t2) e
+| sterm_red_redex : forall env t1 t2, sterm_red env (sapp (slam t1) t2) (ssubstb 0 (sevar (length env)) t1) (t2 :: nil).
+
+Inductive sterme_red : list sterm -> list sitem -> list sitem -> Prop :=
+| sterme_red_promote : forall env t rest, sterme_red env (sitem1 t :: rest) (sitem2 t t :: rest)
+| sterme_red_env : forall env si e1 e2, sterme_red (env ++ readitem si :: nil) e1 e2 -> sterme_red env (si :: e1) (si :: e2)
+| sterme_red_red1 :
+    forall env t1 t2 e rest,
+      sterm_red env t1 t2 e ->
+      sterme_red env (sitem1 t1 :: rest) (map sitem1 e ++ sitem1 t2 :: seshifte (length env) (length e) rest)
+| sterme_red_red2 :
+    forall env t1 t2 t3 e rest,
+      sterm_red env t1 t2 e ->
+      sterme_red env (sitem2 t3 t1 :: rest) (map sitem1 e ++ sitem2 t3 t2 :: seshifte (length env) (length e) rest).
